second

Test/civl/inductive-sequentialization/snapshot-scatter-gather.bpl
@@ -17,12 +17,12 @@ const n: int;
 axiom n >= 1;
 
 var {:layer 0,2} mem: [int]StampedValue;
-var {:layer 0,2} r1: [Tid][int]StampedValue;  
 var {:linear} {:layer 0,2} pSet: Set Permission;
 var {:layer 0,2} channels: [Tid](Option [int]StampedValue);
+var {:layer 0,1} snapshots: [Tid][int]StampedValue;  
 
 function {:inline} WholeTidPermission(tid: Tid): Set Permission {
-    Set((lambda {:pool "D"} x: Permission :: x->tid == tid && (1 <= x->mem_index) && (x->mem_index <= n)))
+    Set((lambda {:pool "D"} x: Permission :: x->tid == tid && 1 <= x->mem_index && x->mem_index <= n))
 }
 
 async action {:layer 1} main_f(tid: Tid, {:linear_in} sps: Set Permission)
@@ -33,24 +33,23 @@ creates read_f;
     assume {:add_to_pool "A", 0, n} true;
     assert sps == WholeTidPermission(tid);
     assert channels[tid] == None();
-    call create_asyncs((lambda pa:read_f :: (1 <= pa->perm->val->mem_index) && (pa->perm->val->mem_index <= n) && pa->perm->val->tid == tid));
+    call create_asyncs((lambda pa:read_f :: 1 <= pa->perm->val->mem_index && pa->perm->val->mem_index <= n && pa->perm->val->tid == tid));
 }
 
 action {:layer 2} main_f'(tid: Tid, {:linear_in} sps: Set Permission)
-modifies r1, pSet, channels;
+modifies pSet, channels;
 {
-    var {:linear} done_set: Set Permission;
+    var snapshot: [int]StampedValue;  
     assume {:add_to_pool "A", 0, n} true;
     assert sps == WholeTidPermission(tid);
     assert channels[tid] == None();
-    havoc r1;
-    assume (forall i:int :: ((1 <= i && i <= n) ==> (r1[tid][i]->ts < mem[i]->ts  || r1[tid][i]== mem[i]))); 
+    assume (forall i:int :: 1 <= i && i <= n ==> (snapshot[i]->ts < mem[i]->ts  || snapshot[i]== mem[i]));
     call Set_Put(pSet, sps);
-    call ChannelSend(tid);
+    call ChannelSend(tid, snapshot);
 }
 
 async action {:layer 1} {:exit_condition Set_IsSubset(WholeTidPermission(perm->val->tid), Set_Add(pSet, perm->val))} read_f({:linear_in} perm: One Permission)
-modifies r1, pSet, channels;
+modifies snapshots, pSet, channels;
 {
     var {:pool "K"} k:int;
     var {:pool "V"} v:Value;
@@ -60,14 +59,14 @@ modifies r1, pSet, channels;
     if (*) {
         assume {:add_to_pool "K", mem[perm->val->mem_index]->ts, k} {:add_to_pool "V", mem[perm->val->mem_index]->value, v} true;
         assume k < mem[perm->val->mem_index]->ts; 
-        r1[perm->val->tid][perm->val->mem_index]:= StampedValue(k, v);
+        snapshots[perm->val->tid][perm->val->mem_index]:= StampedValue(k, v);
     } else {
-        r1[perm->val->tid][perm->val->mem_index]:= mem[perm->val->mem_index];
+        snapshots[perm->val->tid][perm->val->mem_index]:= mem[perm->val->mem_index];
     }
     call One_Put(pSet, perm);
 
     if (Set_IsSubset(WholeTidPermission(perm->val->tid), pSet)) {
-        call ChannelSend(perm->val->tid);
+        call ChannelSend(perm->val->tid, snapshots[perm->val->tid]);
     }
 }
 
@@ -80,22 +79,22 @@ modifies mem;
 }
 
 action {:layer 1} Inv_f(tid: Tid, {:linear_in} sps: Set Permission)
-modifies r1, pSet, channels;
+modifies snapshots, pSet, channels;
 creates read_f;
 {
     var {:pool "A"} j: int;
-    var {:linear} sps2: Set Permission;
+    var {:linear} sps': Set Permission;
     var {:linear} done_set: Set Permission;
     var choice: read_f;
-    sps2 := sps;
     assert sps == WholeTidPermission(tid);
     assert channels[tid] == None();
     assume {:add_to_pool "A", 0, j+1, n} 0 <= j && j <= n;
-    havoc r1;
-    assume (forall i:int :: ((1 <= i && i <= j) ==> (r1[tid][i]->ts < mem[i]->ts || r1[tid][i]== mem[i]))); 
+    havoc snapshots;
+    assume (forall i:int :: 1 <= i && i <= j ==> (snapshots[tid][i]->ts < mem[i]->ts || snapshots[tid][i]== mem[i]));
 
     assume {:add_to_pool "D", Permission(tid, n)} true;
-    call done_set := Set_Get(sps2, (lambda {:pool "D" } x: Permission :: (x->tid == tid) && (1 <= x->mem_index) && (x->mem_index <= j)));
+    sps' := sps;
+    call done_set := Set_Get(sps', (lambda {:pool "D" } x: Permission :: x->tid == tid && 1 <= x->mem_index && x->mem_index <= j));
   
     call Set_Put(pSet, done_set);
     if (j < n) {
@@ -104,23 +103,22 @@ creates read_f;
         call create_asyncs((lambda {:pool "C" } pa:read_f :: j+1 <=  pa->perm->val->mem_index && pa->perm->val->mem_index <= n && pa->perm->val->tid == tid));
         call set_choice(choice);
     } else {
-        call ChannelSend(tid);
+        call ChannelSend(tid, snapshots[tid]);
     }
 }
 
-action {:layer 1,2} ChannelSend(tid: Tid)
+action {:layer 1,2} ChannelSend(tid: Tid, snapshot: [int]StampedValue)
 modifies channels;
 {
     assert Set_IsSubset(WholeTidPermission(tid), pSet);
     assert channels[tid] == None();
-    channels[tid] := Some(r1[tid]);
+    channels[tid] := Some(snapshot);
 }
 
-action {:layer 1,2} ChannelReceive(tid: Tid) returns (r: [int]StampedValue)
+action {:layer 1,2} ChannelReceive(tid: Tid) returns (snapshot: [int]StampedValue)
 modifies channels;
 {
-    assert Set_IsSubset(WholeTidPermission(tid), pSet);
-    assert channels[tid] != None();
-    r := channels[tid]->t;
+    assume channels[tid] != None();
+    snapshot := channels[tid]->t;
     channels[tid] := None();
 }
